FokkerChallenge.lean
@@ -15,6 +15,8 @@ import FokkerChallenge.EnhancedCslib.FvarSubset
 import FokkerChallenge.EnhancedCslib.ReflTransGenWithSteps
 import FokkerChallenge.EnhancedCslib.LeftMost
 import FokkerChallenge.EnhancedCslib.Closedunderapp
+import FokkerChallenge.EnhancedCslib.FlipApp
+import FokkerChallenge.EnhancedCslib.List
 import FokkerChallenge.Decider.NoDuplicate
 import FokkerChallenge.Decider.EveryBvarUsed
 import FokkerChallenge.Decider.All0
