FokkerChallenge/EnhancedCslib/FlipApp.lean
@@ -1,0 +1,26 @@
+import Cslib.Languages.LambdaCalculus.LocallyNameless.Untyped.Basic
+import Cslib.Languages.LambdaCalculus.LocallyNameless.Untyped.FullBeta
+
+namespace Cslib
+
+namespace LambdaCalculus.LocallyNameless.Untyped.Term
+
+lemma step_flip_app_l {M M'} {Ns : List (Term String)} (steps : M ⭢βᶠ M') (lc_Ns : ∀ N ∈ Ns, LC N) :
+    Ns.foldl (flip app) M ⭢βᶠ Ns.foldl (flip app) M' := by
+  induction Ns generalizing M M' with
+  | nil => grind
+  | cons head tail ih =>  simp [flip]
+                          apply ih <;> grind
+
+lemma steps_flip_app_l {M M'} {Ns : List (Term String)} (steps : M ↠βᶠ M') (lc_Ns : ∀ N ∈ Ns, LC N) :
+    Ns.foldl (flip app) M ↠βᶠ Ns.foldl (flip app) M' := by
+  induction steps <;> grind [step_flip_app_l]
+
+lemma flip_app_fv {M} {Ns : List (Term String)}:
+  (Ns.foldl (flip app) M).fv = (Ns.map fv).foldl Union.union M.fv := by
+    induction Ns generalizing M with
+    | nil => grind
+    | cons head tail ih =>
+      simp [flip]
+      specialize @ih (head.app M)
+      grind
